attempt collision bound proof on one call, not sure whether to remove oracle first or whether to remove key update (with blists) first. they seem to depend on each other. try reusing PRF_DRBG proof for the loop--not sure how to do it if the key needs the last output (does that matter?). and will the Permutation postcondition be strong enough?

src/examples/HMAC_DRBG_nonadaptive.v
@@ -5448,6 +5448,204 @@ Proof.
     omega. fcf_spec_ret.
 Qed.
 
+(* --- try to get rid of oracle first *)
+
+Definition Gi_rb_bad_no_oracle' (k v : Bvector eta) (blocks : nat) : Comp bool :=
+  [bits, kv_state, otherInputs] <-$3 GenUpdate_rb_inputs (k, v) blocks;
+  [v', keyInput] <-2 otherInputs;
+  let firstInput := to_list v in (* fixed *)
+  let nextInput := to_list v' in (* extra input to refresh the v *)
+  let outputsAsInputs := firstn (blocksPerCall - 1) (map (fun v => to_list v) bits) in (* only the outputs (so v' is not duplicated) -- we need to remove the last output because that isn't used as an input. OR we can leave it in and get a slightly worse bound. *)
+  ret (hasDups _ (keyInput :: firstInput :: nextInput :: outputsAsInputs)).
+
+Import Permutation.
+
+(* matching PRF_DRBG_f_bad but returning the last result. ok if that's a bvector eta? *)
+Fixpoint Gen_loop_rb_blist (v : Bvector eta) (n : nat)
+  : Comp (list Blist * Bvector eta) := 
+  match n with
+  | O => ret (nil, v)
+  | S n' =>
+    v' <-$ {0,1}^eta;
+    [bits, v''] <-$2 Gen_loop_rb_blist v' n';
+    ret (to_list v' :: bits, v'')
+  end.
+
+(* emulates PRF_DRBG_f_bad_spec *)
+Theorem PRF_DRBG_f_bad_spec_withv : forall n v (ls : list (Blist * Bvector eta)),
+
+    comp_spec (fun (x1 : list (Bvector eta) * Bvector eta * list (Blist * Bvector eta)) (x2 : list Blist * Bvector eta) =>
+                  Permutation (fst (split (snd x1))) ((fst (split ls)) ++ fst x2))
+
+              (* TODO need to prove output keys eq? *)
+   (* comp_spec *)
+   (*   (fun (x : list (Bvector eta) * Bvector eta * list (Blist * Bvector eta)) *)
+   (*      (y : list (Bvector eta) * Bvector eta) => fst x = y /\ True) *)
+
+     (* ((PRF_DRBG_f_G2 v n) _ _ *)
+     (*    (fun (ls : list (D * Bvector eta)) (a : D) => *)
+     (*     x <-$ { 0 , 1 }^eta; ret (x, (a, x) :: ls)) *)
+     (*    ls) *)
+     ((Gen_loop_oc v n) (list (Blist * Bvector eta))
+        (list_EqDec (pair_EqDec eqdbl (Bvector_EqDec eta)))
+        (fun (state : list (Blist * Bvector eta)) (input : Blist) =>
+         output <-$ { 0 , 1 }^eta; ret (output, (input, output) :: state)) ls)
+        (* ((to_list v, a) :: init)) *)
+
+     (* (PRF_DRBG_f_bad v n). *)
+     (Gen_loop_rb_blist v n).
+Proof.
+  induction n; intuition; simpl in *.
+  fcf_simp.
+  fcf_spec_ret.
+  simpl.
+  rewrite app_nil_r.
+  apply Permutation_refl.
+
+  fcf_inline_first.
+  fcf_skip.
+  fcf_skip.
+  fcf_simp.
+  fcf_spec_ret.
+  simpl in H4.
+  simpl.
+  destruct (split ls).
+  simpl in H4. simpl.
+  (* wait, the two of them are defined totally differently... gen_loop_rb_blist and prf_drbg_f_bad *)
+  eapply Permutation_trans.
+  apply H4.
+  (* apply Permutation_cons_app. *)
+  (* apply Permutation_refl. *)
+Admitted.
+
+Lemma Gi_rb_collisions_remove_oracle_first : forall k v blocks init,
+  comp_spec eq
+     (a <-$
+      (GenUpdate_oc (k, v) blocks) (list (Blist * Bvector eta))
+        (list_EqDec (pair_EqDec eqdbl (Bvector_EqDec eta))) rb_oracle init;
+      [_, init']<-2 a; ret hasInputDups init') 
+     (Gi_rb_bad_no_oracle' k v blocks).
+Proof.
+  intros k v blocks init.
+  unfold GenUpdate_oc.
+  unfold Gi_rb_bad_no_oracle'. simplify.
+  unfold rb_oracle. simplify.
+  fcf_skip_eq.
+  simplify.
+  (* Error: Impossible to unify "(list (Bvector eta) * Bvector eta)%type" with
+ "(list (Bvector eta) * Bvector eta * list (Blist * Bvector eta))%type". *)
+  fcf_skip.
+  (* instantiate (1 := (fun x y => fst (split (snd x)) = map (fun c  => to_list c) (fst y))). *)
+  instantiate (1 := (fun x y => fst x = y /\ True)).
+  {
+    Print Gen_loop_rb_intermediate.
+    revert k v blocks init a. clear H.
+    induction blocks as [ | blocks']; intros; simplify.
+    (* need to generalize RB state? *)
+    - fcf_spec_ret.
+    (* - fcf_skip_eq. fcf_skip. (* eapply IHblocks'. *) *)
+    - admit.
+  }
+  simpl in *. 
+  simplify.
+  fcf_skip_eq.
+  simplify.
+  inversion H3. subst.
+  fcf_spec_ret.
+  unfold hasInputDups. simpl. 
+  unfold split. 
+  simplify.                     (* why doesn't simpl work... *)
+  apply Permutation_hasDups.
+  constructor.
+
+  (* can I prove the two postconditions separately and then conjoin them?? *)
+  SearchAbout (comp_spec (fun x y => _ /\ _) _ _).
+  (* TODO make it generic *)
+  assert (comp_spec_and : forall P Q a b, comp_spec P a b -> comp_spec Q a b -> comp_spec (fun c d => P c d /\ Q c d) a b).
+  { intros. admit. }
+    
+
+  admit.
+  (* don't do f_equal, we want to apply Permutation_hasDups *)
+  (* Transparent hasDups. *)
+  (* remember (to_list v *)
+  (*        :: to_list a *)
+  (*           :: firstn (blocksPerCall - 1) *)
+  (*                (map (fun v0 : Vector.t bool eta => to_list v0) l)) as inner. *)
+  (* simpl. *)
+  (* f_equal. f_equal. *)
+
+  (* i can't use PRF_DRBG_f_G2 as-is because it doesn't return the last bitvector, and i need the last bitvector as the k input? or could i replace it with anything? *)
+  (* also injD is to_list *)
+
+Print rb_oracle.
+(* actually the order is wrong... rb_oracle conses each new query into the beginning *)
+(* it should be (rev firstn map to_list l) ++ [to_list a] ++ [to_list v] *)
+(* or maybe i should reason about permutations... *)
+(* also, yeah, i need to add rb_oracle state to the postcondition for loop *)
+(* also, if i prove permutation here, will that allow me to prove eq later? probably yes, eq is on hasDups *)
+(* then I need to use a theorem on hasDups $ perm l = hasDups l *)
+(* can i apply PRF_DRBG_f_bad_spec here?? and if I do, is that postcondition helpful? and can I directly apply it, or do I need to copy-and-paste the proof? *)
+
+  (* v = the input v, a = output of rb_oracle v *)
+  (* the `to_list v` got stuck in the rb_oracle's input state in gen_loop_oc *)
+(* this should be the postcondition!... is it true? what happened to my actual postcondition? *)
+  (* the second half worked (the last v that each loop is the output to each k-sampling) *)
+  (* the first half was thrown away (hasInputDups ignores the bits output) *)
+Qed.
+
+(* --- *)
+
+(* maybe I should remove k entirely? *)
+Definition GenUpdate_oc_noKsample (state : KV) (n : nat) :
+  OracleComp (list bool) (Bvector eta) (list (Bvector eta) * KV) :=
+  [k, v_0] <-2 state;
+  v <--$ (OC_Query _ (to_list v_0)); (* ORACLE USE *)
+  [bits, v'] <--$2 Gen_loop_oc v n;
+  $ ret (bits, (k, v')).
+
+(* try removing k first, but i lose information about the length of the list... *)
+Lemma Gi_rb_collisions_remove_k_first : forall k v blocks init,
+  comp_spec eq
+     (a <-$
+      (GenUpdate_oc (k, v) blocks) (list (Blist * Bvector eta))
+        (list_EqDec (pair_EqDec eqdbl (Bvector_EqDec eta))) rb_oracle init;
+      [_, init']<-2 a; ret hasInputDups init') 
+     (a <-$
+      (GenUpdate_oc_noKsample (k, v) blocks) (list (Blist * Bvector eta))
+        (list_EqDec (pair_EqDec eqdbl (Bvector_EqDec eta))) rb_oracle init;
+      [_, init']<-2 a; ret hasInputDups init').
+Proof.
+  intros k v blocks init.
+  unfold GenUpdate_oc.
+  unfold GenUpdate_oc_noKsample. simplify.
+  unfold rb_oracle. simplify.
+  fcf_skip_eq. simplify.
+  (* maybe prove something about gen_loop and how its output is eq to comp_map here? *)
+  (* or really, oracleCompMap... *)
+  (* proving a stronger postcondition than eq *)
+  (* eapply comp_spec_seq. apply true. apply true. *)
+ (* instantiate (1 := (fun x y => x = y /\ True )). *)
+  (* admit. *)
+  (* reasoning about split of anything is annoying. maybe get rid of the outputs first/? *)
+  (* or: get rid of oracle, then prove that it's hasDups eqdbl keyInput :: map to_list compMap... *)
+SearchAbout Forall.
+Print GenUpdate_oc.
+
+  fcf_skip. simplify.
+  fcf_irr_l. simplify.
+  unfold hasInputDups.
+  simplify.
+  fcf_spec_ret.
+  Transparent hasDups. simplify.
+  (* uh oh, I lost information about all elements of l having the same length and b1 having the same length as them *)
+(* i have the `to_list b1` (now i need to reason about `Bvector eta`s??) *)
+(* maybe i want a postcondition on `l = map to_list ...` *)
+(* in that case, I should simplify gen_loop first *)
+(* there's to_list_length *)
+
+Admitted.
+
 Lemma Gi_rb_collisions_inner_eq : forall k v blocks init,
   comp_spec eq
      (a <-$
@@ -5457,8 +5655,15 @@ Lemma Gi_rb_collisions_inner_eq : forall k v blocks init,
 Proof.
   intros k v blocks init.
   unfold GenUpdate_oc.
-  simplify.
   unfold compMap_v.
+
+  (* why not get rid of the oracle computation in GenUpdate_oc? *)
+  Print Gi_rb_bad_no_oracle.
+  Print GenUpdate_rb_inputs.
+  (* i should also get rid of that key line ASAP, and convert everything to vectors *)
+  (* what about reasoning about permutations? *)
+
+  simplify.
   Transparent compMap.
   unfold rb_oracle. simplify.
   fcf_irr_l.
